sliding bloom filter model

newLibrary/slidingBloomFilter.dfy
@@ -21,3 +21,81 @@
                 insert(k) @ t ==> forall t' :: 
                     (t < t' <= t + paneCycleTime)  ==> (query(k) @ t == true)
 */
+
+include "verifiableLucid.dfy"
+
+module SlidingBloomFilter refines VerifiableLucid {
+    datatype Event = 
+        | insert(key : uint32)
+        | query(key: uint32)
+
+    class Program ... {
+        const nRows : uint32 := 32
+        const seed0 : uint32 := 7
+        const seed1 : uint32 := 13
+
+        // interval between switching panes
+        // we need to see at least nRows packets during this 
+        // interval, to clear each entry in the expired pane.
+        // lets say its 10 * nRows, which means that 
+        // we must see 1 packet every 10 time units.
+        const tinterval : uint32 := 10 * nRows
+
+        var activePane : LArray<uint32> // which pane is active
+        var clearIdx   : LArray<uint32> // current index to clear
+        // Three panes with 2 columns each
+        var p0col0 : LArray<uint32>  // active pane, column 0
+        var p0col1 : LArray<uint32>  // active pane, column 1
+        var p1col0 : LArray<uint32>  // maintaining pane, column 0
+        var p1col1 : LArray<uint32>  // maintaining pane, column 1
+        var p2col0 : LArray<uint32>  // clearing pane, column 0
+        var p2col1 : LArray<uint32>  // clearing pane, column 1
+        
+        constructor ()
+            ensures fresh(activePane)
+            ensures fresh(clearIdx)
+            ensures fresh(p0col0) && fresh(p0col1)
+            ensures fresh(p1col0) && fresh(p1col1)
+            ensures fresh(p2col0) && fresh(p2col1)
+            ensures activePane.cells == [0]
+            ensures clearIdx.cells == [0]
+            ensures p0col0.cells == zeros(nRows) && p0col1.cells == zeros(nRows)
+            ensures p1col0.cells == zeros(nRows) && p1col1.cells == zeros(nRows)
+            ensures p2col0.cells == zeros(nRows) && p2col1.cells == zeros(nRows)
+            ensures fresh(this)
+        {
+            activePane := new LArray<uint32>.Create(1, 0);
+            clearIdx := new LArray<uint32>.Create(1, 0);
+            p0col0 := new LArray<uint32>.Create(nRows, 0);
+            p0col1 := new LArray<uint32>.Create(nRows, 0);
+            p1col0 := new LArray<uint32>.Create(nRows, 0);
+            p1col1 := new LArray<uint32>.Create(nRows, 0);
+            p2col0 := new LArray<uint32>.Create(nRows, 0);
+            p2col1 := new LArray<uint32>.Create(nRows, 0);
+        }
+
+
+
+        function hash(seed : uint32, key : uint32) : uint32
+            ensures 0 <= hash(seed, key) < nRows
+        {
+            to_uint32((seed + key) % nRows)
+        }
+
+        /*
+        query:
+            ci := clearIndex.update(sat_incr);
+            if (activePane == 0) {
+                read(p0);
+                read(p1);
+                write(p2, ci, 0);                
+
+            }
+
+        */
+
+
+
+    }    
+
+}
